Equip Block with auxiliary BlockSource and QC types.

Structures/Blocks.v
@@ -1,5 +1,5 @@
 From mathcomp.ssreflect
-Require Import ssreflect ssrbool ssrnat eqtype ssrfun seq path.
+Require Import ssreflect ssrbool ssrnat eqtype fintype ssrfun seq path.
 Require Import Eqdep.
 From fcsl
 Require Import pred prelude ordtype pcm finmap unionmap heap.
@@ -9,10 +9,75 @@ Set Implicit Arguments.
 Unset Strict Implicit.
 Unset Printing Implicit Defensive.
 
+Section BlockSource.
+
+Variables (Address: finType) (VProof: eqType).
+
+Record BlockSource := mkBS {
+                          author: Address;
+                          signature: VProof;
+                        }.
+
+Definition eq_block_source (b b' : BlockSource) :=
+  match b, b' with
+  | mkBS auth sig, mkBS auth' sig' =>
+    (auth == auth') && (sig == sig')
+  end.
+
+Lemma eq_block_sourceP: Equality.axiom eq_block_source.
+Proof.
+move => bs bs'.
+apply (iffP idP)=> [|->]; last by case bs'=>a' s' //=; rewrite ?eqxx //.
+case bs=> a s; case bs'=> a' s'; [case/andP; move/eqP ->].
+by move/eqP->.
+Qed.
+
+
+Canonical BlockSource_eqMixin :=
+  Eval hnf in EqMixin eq_block_sourceP.
+Canonical BlockSource_eqType :=
+  Eval hnf in EqType BlockSource BlockSource_eqMixin.
+
+End BlockSource.
+
+Section QuorumCert.
+
+Variable Hash: ordType.
+Variable VProof: eqType.
+
+Record QuorumCert := mkQC {
+                      block_hash: Hash;
+                      executed_hash: Hash;
+                      block_round: nat;
+                      parent_block_hash: Hash;
+                      parent_block_round: nat;
+                      grandparent_block_hash: Hash;
+                      grandparent_block_round: nat;
+                      votes: seq VProof;
+                    }.
+
+Definition eq_quorum_cert (qc qc': QuorumCert) :=
+  match qc, qc' with
+  | mkQC bh eh br pbh pbr gpbh gpbr v, mkQC bh' eh' br' pbh' pbr' gpbh' gpbr' v' =>
+    [&& bh == bh', eh == eh', br == br', pbh == pbh', pbr == pbr', gpbh == gpbh', gpbr == gpbr' & v == v']
+  end.
+
+Lemma eq_qcP: Equality.axiom eq_quorum_cert.
+ Proof.
+move => qc qc'; apply: (iffP idP) => [| ->].
+- case qc=> bh eh br ph pr gph gpr v;
+  case qc'=> bh' eh' br' ph' pr' gph' gpr' v' /=; do? [case/andP; move/eqP ->]; by move/eqP ->.
+- by case qc'=> bh' eh' br' ph' pr' gph' gpr' v' //=; do? rewrite eqxx.
+Qed.
+
+Canonical QC_eqMixin := Eval hnf in EqMixin eq_qcP.
+Canonical QC_eqType := Eval hnf in EqType QuorumCert QC_eqMixin.
+
+End QuorumCert.
+
 Section BlockType.
 
-
-Variables (Hash NodeTime : ordType) (Command VProof BlockSource : eqType).
+Variables (Hash NodeTime : ordType) (Command VProof : eqType) (Address: finType).
 
 Record Block :=
   mkB {
@@ -24,8 +89,8 @@ Record Block :=
     time: NodeTime;
     round: nat;
     (* Parent's QC information *)
-    proof : VProof;
-    source: BlockSource;
+    proof : QuorumCert Hash VProof;
+    source: BlockSource Address VProof;
   }.
 
 Definition eq_block (b b' : Block) :=
